implicit arguments for Tnil (to do: Tcons,  etc.)

theories/ordinals/Ackermann/LNN.v
@@ -18,18 +18,18 @@ Definition Terms := Terms LNN.
 Definition SysPrf := SysPrf LNN.
 
 Definition Plus (x y : Term) : Term :=
-  @apply LNN Plus (Tcons LNN 1 x (Tcons LNN 0 y (Tnil LNN))).
+  @apply LNN Plus (Tcons LNN 1 x (Tcons LNN 0 y (Tnil))).
 
 Definition Times (x y : Term) : Term :=
-  @apply LNN Times (Tcons LNN 1 x (Tcons LNN 0 y (Tnil LNN))).
+  @apply LNN Times (Tcons LNN 1 x (Tcons LNN 0 y (Tnil))).
 
 Definition Succ (x : Term) : Term :=
-  @apply LNN Succ (Tcons LNN 0 x (Tnil LNN)).
+  @apply LNN Succ (Tcons LNN 0 x (Tnil)).
 
-Definition Zero : Term := @apply LNN Zero (Tnil LNN).
+Definition Zero : Term := @apply LNN Zero (Tnil).
 
 Definition LT (x y : Term) : Formula :=
-  @atomic LNN LT (Tcons LNN 1 x (Tcons LNN 0 y (Tnil LNN))). 
+  @atomic LNN LT (Tcons LNN 1 x (Tcons LNN 0 y (Tnil))). 
 (* end snippet Instantiations *)
 
 Lemma LNN_dec : language_decidable LNN.
@@ -247,10 +247,10 @@ Lemma eqPlus (T : System) (a b c d : Term):
  SysPrf T (equal c d) -> SysPrf T (equal (Plus a c) (Plus b d)).
 Proof.
   intros H H0; unfold Plus; apply (equalFunction); simpl.  
-  destruct (consTerms LNN 1 (Tcons _ 1 a (Tcons _ 0 c (Tnil _))))
+  destruct (consTerms LNN 1 (Tcons _ 1 a (Tcons _ 0 c (Tnil))))
     as [(a0, b0) p]. 
   simpl; 
-    destruct  (consTerms LNN 1 (Tcons _ 1 b (Tcons _ 0 d (Tnil _))))
+    destruct  (consTerms LNN 1 (Tcons _ 1 b (Tcons _ 0 d (Tnil))))
     as [(a1, b1) p0].
   simpl; destruct  (consTerms LNN 0 b0) as [(a2, b2) p1].
   simpl; destruct  (consTerms LNN 0 b1) as [(a3,b3) p2].
@@ -273,9 +273,9 @@ Lemma eqTimes (T : System) (a b c d : Term):
 Proof.
   intros H H0; unfold Times; apply (equalFunction LNN).
   simpl; 
-    destruct (consTerms LNN 1 (Tcons _ 1 a (Tcons _ 0 c (Tnil _))))
+    destruct (consTerms LNN 1 (Tcons _ 1 a (Tcons _ 0 c (Tnil))))
     as [(a0, b0) p].
-  simpl; destruct (consTerms LNN 1 (Tcons _ 1 b (Tcons _ 0 d (Tnil _))))
+  simpl; destruct (consTerms LNN 1 (Tcons _ 1 b (Tcons _ 0 d (Tnil))))
     as [(a1, b1) p0].
   simpl; destruct  (consTerms LNN 0 b0) as [(a2, b2) p1].
   simpl; induction (consTerms LNN 0 b1) as [(a3,b3) p2].
@@ -301,9 +301,9 @@ Lemma eqSucc (T : System) (a b : Term):
   SysPrf T (equal a b) -> SysPrf T (equal (Succ a) (Succ b)).
 Proof.
   intro H; unfold Succ; apply (equalFunction LNN).
-  simpl; destruct (consTerms LNN 0 (Tcons _ 0 a (Tnil _)))
+  simpl; destruct (consTerms LNN 0 (Tcons _ 0 a (Tnil)))
     as [(a0, b0) p].
-  simpl; destruct  (consTerms LNN 0 (Tcons LNN 0 b (Tnil LNN)))
+  simpl; destruct  (consTerms LNN 0 (Tcons LNN 0 b (Tnil)))
     as [(a1, b1) p0].
   simpl; repeat split.
   simpl in p.
@@ -318,9 +318,9 @@ Lemma eqLT (T : System) (a b c d : Term):
   SysPrf T (equal c d) -> SysPrf T (iffH (LT a c) (LT b d)).
 Proof.
   intros H H0; unfold LT; apply (equalRelation LNN).
-  simpl;  destruct  (consTerms LNN 1 (Tcons _ 1 a (Tcons _ 0 c (Tnil _))))
+  simpl;  destruct  (consTerms LNN 1 (Tcons _ 1 a (Tcons _ 0 c (Tnil))))
     as [(a0, b0) p].
-  simpl; destruct (consTerms LNN 1 (Tcons _ 1 b (Tcons _ 0 d (Tnil _))))
+  simpl; destruct (consTerms LNN 1 (Tcons _ 1 b (Tcons _ 0 d (Tnil))))
     as [(a1, b1) p0].
   simpl; destruct (consTerms LNN 0 b0) as [(a2, b2) p1]. 
 
