theories/ordinals/Ackermann/LNT.v
@@ -17,15 +17,15 @@ Definition Terms := Terms LNT.
 Definition SysPrf := SysPrf LNT.
 
 Definition Plus (x y : Term) : Term :=
-  @apply LNT Plus (Tcons LNT 1 x (Tcons LNT 0 y (Tnil LNT))).
+  @apply LNT Plus (Tcons LNT 1 x (Tcons LNT 0 y (Tnil))).
 
 Definition Times (x y : Term) : Term :=
-  @apply LNT Times (Tcons LNT 1 x (Tcons LNT 0 y (Tnil LNT))).
+  @apply LNT Times (Tcons LNT 1 x (Tcons LNT 0 y (Tnil))).
 
 Definition Succ (x : Term) : Term :=
-  @apply LNT Succ (Tcons LNT 0 x (Tnil LNT)).
+  @apply LNT Succ (Tcons LNT 0 x (Tnil)).
 
-Definition Zero : Term := @apply LNT Zero (Tnil LNT).
+Definition Zero : Term := @apply LNT Zero (Tnil).
 
 Lemma LNT_dec : language_decidable LNT.
 Proof. split; decide equality. Qed.
@@ -243,8 +243,8 @@ Proof.
   intros H H0; unfold Plus.
   apply (equalFunction LNT).
   simpl in |- *.
-  destruct (consTerms LNT 1 (Tcons LNT 1 a (Tcons LNT 0 c (Tnil LNT))))as [(a0,b0) p].
-  simpl; destruct (consTerms LNT 1 (Tcons _ 1 b (Tcons _ 0 d (Tnil _)))) 
+  destruct (consTerms LNT 1 (Tcons LNT 1 a (Tcons LNT 0 c (Tnil))))as [(a0,b0) p].
+  simpl; destruct (consTerms LNT 1 (Tcons _ 1 b (Tcons _ 0 d (Tnil)))) 
     as [(a1,b1) p0]. 
   simpl in |- *.
   destruct (consTerms LNT 0 b0) as [(a2,b2) p1]. 
@@ -274,9 +274,9 @@ Lemma eqTimes  (T : System) (a b c d : Term):
 Proof.
   intros H H0; unfold Times in |- *.
   apply (equalFunction LNT); simpl in |- *.
-  destruct (consTerms LNT 1 (Tcons LNT 1 a (Tcons LNT 0 c (Tnil LNT))))as [(a0,b0) p].
+  destruct (consTerms LNT 1 (Tcons LNT 1 a (Tcons LNT 0 c (Tnil))))as [(a0,b0) p].
   simpl in |- *.
-  destruct (consTerms LNT 1 (Tcons LNT 1 b (Tcons LNT 0 d (Tnil LNT)))) as [(a1,b1) p0].
+  destruct (consTerms LNT 1 (Tcons LNT 1 b (Tcons LNT 0 d (Tnil)))) as [(a1,b1) p0].
   simpl; destruct (consTerms LNT 0 b0) as [(a2,b2) p1].
   simpl ; destruct (consTerms LNT 0 b1) as [(a3,b3) p2].
   simpl in |- *; repeat split.
@@ -302,9 +302,9 @@ Lemma eqSucc (T : System) (a b : Term):
 Proof.
   intros H; unfold Succ in |- *; apply (equalFunction LNT).
   simpl in |- *.
-  destruct (consTerms LNT 0 (Tcons LNT 0 a (Tnil LNT))) as [(a0,b0) p].
+  destruct (consTerms LNT 0 (Tcons LNT 0 a (Tnil))) as [(a0,b0) p].
   simpl in |- *;
-destruct (consTerms LNT 0 (Tcons LNT 0 b (Tnil LNT))) as [(a1,b1) p0].
+destruct (consTerms LNT 0 (Tcons LNT 0 b (Tnil))) as [(a1,b1) p0].
   simpl in |- *; repeat split.
   - simpl in p.
     inversion p.
