theories/ordinals/Ackermann/fol.v
@@ -725,3 +725,4 @@ Arguments var {L} _.
 Arguments atomic {L} _ _.
 Arguments apply {L} _ _.
 Arguments ifThenElseH {L} _ _ _.
+Arguments Tnil {L}.
